ztest.sml
@@ -1408,6 +1408,196 @@ val Lez_def = qdefine_psym ("Lez",[‘z1:mem(Z)’,‘z2:mem(Z)’])
 ‘!a b c d.Repz(z1) = Zc(a,b) & Repz(z2) = Zc(c,d) ==>
  Le(Add(a,d),Add(b,c))’ |> gen_all |> store_as "Lez_def";
 
+(*
+val iscoPr_def = qdefine_psym("iscoPr",[‘i1:A->AB’,‘i2:B->AB’])
+‘!X f:A->X g:B->X.?!fg:AB->X.fg o i1 = f & fg o i2 = g’
+|> qgenl [‘A’,‘B’,‘AB’,‘i1’,‘i2’]
+|> store_as "iscoPr_def";
+
+
+
+val iscoPr_ex = prove_store("iscoPr_ex",
+e0
+cheat
+(form_goal “!A B.?AB i1:A->AB i2:B->AB.iscoPr(i1,i2)”));
+
+
+
+val coPo_def = iscoPr_ex |> spec_all 
+                         |> qSKOLEM "+" [‘A’,‘B’] |> gen_all
+                         |> store_as "coPo_def";
+
+val i1_def = coPo_def |> spec_all 
+                      |> qSKOLEM "i1" [‘A’,‘B’] |> gen_all
+                      |> store_as "i1_def";
+
+val i2_def = i1_def |> spec_all |> qSKOLEM "i2" [‘A’,‘B’] |> gen_all
+                    |> store_as "i2_def";
+
+val coPa_def = i2_def |> rewr_rule[iscoPr_def] |> spec_all
+                      |> uex_expand 
+                      |> qSKOLEM "coPa" [‘f’,‘g’]
+                      |> gen_all
+                      |> store_as "coPa_def";
+
+val r2f_def = proved_th $
+e0
+cheat
+(form_goal “!R:A~>B. ?!f:A * B -> 1+1.
+ !a b. App(f,Pair(a,b)) = App(i2(1,1),dot)  <=> Holds(R,a,b)”)
+|> spec_all |> uex2ex_rule |> qSKOLEM "r2f" [‘R’] |> gen_all
+
+val true_def = qdefine_fsym("true",[]) ‘App(i2(1,1),dot)’
+
+val id_ER = prove_store("id_ER",
+e0
+(rw[id_def,ER_def,Refl_def,Sym_def,Trans_def] >> rpt strip_tac >> arw[])
+(form_goal “!A. ER(id(A))”));
+
+
+(*
+val le0_def = qdefine_psym ("le0",[‘ab:mem(N * N)’,‘cd:mem(N * N)’])
+‘Le(Add(Fst(ab),Snd(cd)),Add(Snd(ab),Fst(cd)))’
+|> gen_all |> conv_rule (depth_fconv no_conv forall_cross_fconv)
+|> rewr_rule[Pair_def'] |> store_as "le0_def"; 
+*)
+
+val ler0_def = proved_th $
+e0
+cheat
+(form_goal “?lef0:(N * N) ~> (N * N). !a b c d.Holds(lef0,Pair(a,b),Pair(c,d))<=> Le(Add(a,d),Add(b,c))
+ ”) |> qSKOLEM "ler0" []
+
+val Sg_Inj = prove_store("Sg_Inj",
+e0
+(rw[Inj_def] >> rw[GSYM IN_EXT_iff,Sg_def] >> rpt strip_tac >>
+ first_x_assum (qspecl_then [‘x1’] assume_tac) >> fs[] )
+(form_goal “!A. Inj(Sg(A))”));
+
+val resp_lef0 = prove_store("resp_lef0",
+e0
+(cheat)
+(form_goal “resp(r2f(ler0), prrel(ZR, ZR), id(1 + 1))”));
+
+val Quo_id_Sg = prove_store("Quo_id_Sg",
+e0
+(rw[Quo_def,GSYM IN_EXT_iff,Sg_def,IN_rsi,id_def] >> 
+ rpt strip_tac >> dimp_tac >> rpt strip_tac(* 2 *)
+ >-- (pop_assum (strip_assume_tac o uex_expand) >>
+ qexists_tac ‘q’ >> arw[] >> strip_tac >> lflip_tac >> rw[]) >>
+ uex_tac >> qexists_tac ‘a’ >> flip_tac >> arw[] >>
+ rpt strip_tac >> first_x_assum (qspecl_then [‘q'’] assume_tac) >> fs[])
+(form_goal “!A.Quo(id(A),Sg(A))”));
+
+val main_LEzf = 
+Quo_fun |> qspecl [‘(N * N) * (N * N)’,‘1+1’,
+                ‘r2f(ler0)’,
+                ‘prrel(ZR,ZR)’,‘id(1+1)’,
+                ‘Z * Z’,‘1+1’,
+                ‘ipow2(iZ,iZ)’,‘Sg(1+1)’]
+|> rewr_rule[addz_conds,id_ER,Sg_Inj,Quo_id_Sg,resp_lef0]
+|> qSKOLEM "LEzf" []
+|> conv_rule (depth_fconv no_conv forall_cross_fconv)
+|> rewr_rule[rext_def]
+
+
+
+val Pow_conj_eq' = proved_th $
+e0
+(rpt gen_tac >> disch_tac >> drule Pow_conj_eq >>
+ dimp_tac >> rpt strip_tac (* 2 *)
+ >-- (first_x_assum drule >> arw[])
+ >-- (first_x_assum drule >> arw[]) >>
+ arw[])
+(form_goal “∀A B s1:mem(Pow(A)) s2:mem(Pow(B)) s3 s4 a0 b0. IN(a0,s1) & IN(b0,s2) ⇒ ( (∀a b. IN(a,s1) & IN(b,s2) ⇔ IN(a,s3) & IN(b,s4)) <=> 
+ s1 = s3 & s2 = s4)”) |> spec_all |> undisch
+|> gen_all |> disch_all|> gen_all
+
+
+val Repz_iff_Asz = prove_store("Repz_iff_Asz",
+e0
+(rpt strip_tac >> dimp_tac >> strip_tac >> arw[] (* 2 *)
+ >-- (irule Repz_eq_eq >> arw[Asz_Repz]) >>
+ pop_assum (assume_tac o GSYM) >> arw[] >>
+ arw[Asz_Repz])
+(form_goal “!z a b. Repz(z) = Zc(a, b) <=> Asz(a,b) = z”));
+
+val ipow2_prrel_ZR = prove_store("ipow2_prrel_ZR",
+e0
+(rw[ipow2_def,GSYM IN_EXT_iff,IN_rsi] >>
+fconv_tac (depth_fconv no_conv forall_cross_fconv) >>
+fconv_tac (depth_fconv no_conv forall_cross_fconv) >> 
+rw[prrel_def,ipow2_def] >>
+rw[GSYM IN_rsi] >>
+qby_tac ‘?xy uv.IN(xy,Repz(z1)) & IN(uv,Repz(z2))’
+>-- (qspecl_then [‘z1’] strip_assume_tac iZ_nonempty >>
+    qspecl_then [‘z2’] strip_assume_tac iZ_nonempty >>
+    rw[Repz_def] >> qexistsl_tac [‘ab’,‘ab'’] >> arw[]) >>
+pop_assum (x_choosel_then ["xy","uv"] assume_tac) >>
+drule Pow_conj_eq' >> rw[GSYM Repz_def] >> 
+first_x_assum (qspecl_then [‘rsi(ZR, Pair(a, b))’,‘rsi(ZR, Pair(c, d))’] assume_tac)>> (*why arw does not work*)
+arw[] >>
+pop_assum mp_tac >> 
+fconv_tac (depth_fconv no_conv forall_cross_fconv) >>
+strip_tac >> arw[] (*why must I use the cross fconv*)>>
+rw[GSYM Zc_def,GSYM ZC_def,Repz_iff_Asz])
+(form_goal
+“App(ipow2(iZ, iZ), Pair(z1, z2)) = rsi(prrel(ZR, ZR), Pair(Pair(a,b),Pair(c,d))) <=> Asz(a,b) = z1 & Asz(c,d) = z2”));
+
+
+val main_LEzf1 = 
+main_LEzf |> rewr_rule[App_App_o,GSYM IN_EXT_iff,IN_rsi,id_def]
+|> rewr_rule[IN_EXT_iff,Sg_def]
+|> rewr_rule[GSYM IN_rsi,IN_EXT_iff]
+
+val main_LEzf2 = prove_store("main_LEzf2",
+e0
+(rpt strip_tac >> 
+ qspecl_then [‘z1’,‘z2’] assume_tac main_LEzf1 >>
+ pop_assum (x_choosel_then ["abcd","tv"] assume_tac) >>
+ qsspecl_then [‘abcd’] (x_choosel_then ["ab","cd"] assume_tac) Pair_has_comp >>
+ qsspecl_then [‘ab’] (x_choosel_then ["a","b"] assume_tac) Pair_has_comp >>
+ qsspecl_then [‘cd’] (x_choosel_then ["c","d"] assume_tac) Pair_has_comp >> 
+ fs[ipow2_prrel_ZR] >> qexistsl_tac [‘a’,‘b’,‘c’,‘d’] >>
+ arw[] >> 
+ first_x_assum (qspecl_then [‘App(LEzf, Pair(z1, z2))’] assume_tac) >>
+ fs[])
+(form_goal “!z1 z2.?a b c d.
+  Asz(a,b) = z1 & Asz(c,d) = z2 & 
+  App(LEzf, Pair(z1, z2)) = App(r2f(ler0), Pair(Pair(a,b),Pair(c,d)))”));
+
+
+val tv_eq_true = prove_store("tv_eq_true",
+e0
+(cheat)
+(form_goal “!tv1 tv2. tv1 = tv2 <=>
+ (tv1 = true <=> tv2 = true)”));
+
+
+val main_LEzf3 = prove_store("main_LEzf3",
+e0
+(rpt strip_tac >> 
+ qspecl_then [‘z1’,‘z2’] strip_assume_tac main_LEzf2 >>
+ qexistsl_tac [‘a’,‘b’,‘c’,‘d’] >> arw[] >>
+ rw[GSYM tv_eq_true])
+(form_goal “!z1 z2.?a b c d.
+  Asz(a,b) = z1 & Asz(c,d) = z2 & 
+  (App(LEzf, Pair(z1, z2)) = true <=> 
+  App(r2f(ler0), Pair(Pair(a,b),Pair(c,d))) = true)”));
+
+val main_LEzf4 = main_LEzf3 |> rewr_rule[true_def,r2f_def,ler0_def] 
+           |> rewr_rule[GSYM true_def]
+
+val f2r_def = proved_th $
+e0
+cheat
+(form_goal “!A B f:A * B -> 1+1.?!R:A~>B.
+ !a b. Holds(R,a,b) <=> App(f,Pair(a,b)) = true”)
+|> spec_all |> uex2ex_rule |> qSKOLEM "f2r" [‘f’] |> gen_all
+
+val LEz_def0 = qdefine_fsym("LEz",[]) ‘f2r(LEzf)’;
+*)
+
 val LEz_def = AX1 |> qspecl [‘Z’,‘Z’] |> fVar_sInst_th “P(a:mem(Z),b:mem(Z))”
                   “Lez(a,b)”
                   |> uex2ex_rule |> qSKOLEM "LEz" []
