ETCSllist.sml
@@ -1,0 +1,714 @@
+
+val BU_ex = prove_store("BU_ex",
+e0
+(cheat)
+(form_goal
+ “!A. ?!BU:Exp(Exp(A,1+1),1+1) -> Exp(A,1+1). 
+  !sss a:1->A. IN(a,BU o sss) <=>
+  ?ss.IN(ss,sss) & IN(a,ss)”));
+ 
+
+val BU_def = BU_ex |> spec_all |> uex2ex_rule 
+                         |> qSKOLEM "BU" [‘A’]
+                         |> gen_all
+                         |> store_as "BU_def"; 
+
+
+val BIGUNION_def = qdefine_fsym("BIGUNION",[‘sss:1->Exp(Exp(A,1+1),1+1)’])
+‘BU(A) o sss’ |> gen_all |> store_as "BIGUNION_def";
+
+
+val IN_BIGUNION = BU_def |> rewr_rule[GSYM BIGUNION_def] 
+                         |> store_as "IN_BIGUNION";
+
+
+(*for every f:Exp(A,1+1) -> Exp(A,1+1), there is a unique predicate coresponds the predicate X ⊆ f X
+
+qform2IL [‘P1:1->Exp(A,2)’] ‘SS(P1,P2)’*)
+
+
+val SSf_IL_uex = prove_store("SSf_IL_uex",
+e0
+(cheat)
+(form_goal “!A f:Exp(A,1+1) ->Exp(A,1+1). ?!p:Exp(A,1+1) -> 1+1.
+ !s:1->Exp(A,1+1). SS(s,f o s) <=> p o s = TRUE”));
+
+val SSf_IL_def = SSf_IL_uex |> spec_all |> uex2ex_rule |> qSKOLEM "SSfIL" [‘f’]
+                            |> gen_all
+
+val gfp_def = qdefine_fsym("gfp",[‘f:Exp(A,1+1) -> Exp(A,1+1)’])
+‘BIGUNION(Tp1(SSfIL(f)))’ |> gen_all 
+
+
+val IN_gfp = prove_store("IN_gfp",
+e0
+(cheat)
+(form_goal “!f:Exp(A,1+1) ->Exp(A,1+1) a. 
+ IN(a,gfp(f)) <=> ?X. SS(X,f o X) & IN(a,X)”));
+
+val weak_coind = prove_store("weak_coind",
+e0
+(rpt strip_tac >> rw[IN_gfp] >>
+ qexists_tac ‘X’ >> arw[])
+(form_goal “!A X:1->Exp(A,1+1) a f.IN(a,X) & SS(X,f o X) ==> IN(a,gfp(f))  ”));
+
+val monotone_def = qdefine_psym("monotone",[‘f:Exp(A,1+1)->Exp(B,1+1)’])
+‘!s1 s2. SS(s1,s2) ==> SS(f o s1, f o s2)’ |> gen_all
+
+
+val SS_gfp_fgfp = prove_store("SS_gfp_fgfp",
+e0
+(rw[SS_def,IN_gfp] >> 
+ rpt strip_tac >>
+ first_assum drule >> fs[monotone_def] >>
+ qsuff_tac ‘SS(f o X,f o gfp(f))’ 
+ >-- (rw[SS_def] >> rpt strip_tac >> first_x_assum irule >> arw[]) >>
+ first_x_assum irule >> 
+ rw[SS_def,IN_gfp] >> rpt strip_tac >>
+ qexists_tac ‘X’ >> arw[])
+(form_goal
+ “monotone(f) ==> SS(gfp(f:Exp(A,1+1) ->Exp(A,1+1)), f o gfp(f))”));
+
+
+val rules0 = prove_store("rule0",
+e0
+(rw[SS_def,IN_gfp] >> rpt strip_tac >>
+ assume_tac SS_gfp_fgfp >> first_x_assum drule >> 
+ qexists_tac ‘gfp(f)’ >> arw[GSYM SS_def] >>
+ rw[IN_gfp] >> qexists_tac ‘f o gfp(f)’ >> arw[] >>
+ fs[monotone_def] >> first_x_assum irule >> arw[])
+(form_goal
+ “monotone(f) ==> SS(f o gfp(f),gfp(f:Exp(A,1+1) ->Exp(A,1+1)))”));
+
+
+val cases0 = prove_store("cases0",
+e0
+(rpt strip_tac >> irule SS_SS_eq >>
+ drule rules0 >> drule SS_gfp_fgfp >> arw[])
+(form_goal “monotone(f) ==> gfp(f:Exp(A,1+1) ->Exp(A,1+1)) =  f o gfp(f)”))
+
+val coind0 = prove_store("coind0",
+e0
+(rpt strip_tac >> rw[SS_def] >> rpt strip_tac >> irule weak_coind >>
+ qexists_tac ‘X’ >> arw[])
+(form_goal “!f:Exp(A,1+1) ->Exp(A,1+1) X. SS(X,f o X) ==> SS(X,gfp(f))”));
+
+
+
+(*
+val lrep_ok_cases =
+   ⊢ ∀a0.
+       lrep_ok a0 ⇔
+       a0 = (λn. NONE) ∨
+       ∃h t. a0 = (λn. if n = 0 then SOME h else t (n − 1)) ∧ lrep_ok t: thm
+val lrep_ok_coind =
+   ⊢ ∀lrep_ok'.
+       (∀a0.
+          lrep_ok' a0 ⇒
+          a0 = (λn. NONE) ∨
+          ∃h t. a0 = (λn. if n = 0 then SOME h else t (n − 1)) ∧ lrep_ok' t) ⇒
+       ∀a0. lrep_ok' a0 ⇒ lrep_ok a0: thm
+val lrep_ok_rules =
+   ⊢ lrep_ok (λn. NONE) ∧
+     ∀h t. lrep_ok t ⇒ lrep_ok (λn. if n = 0 then SOME h else t (n − 1)): thm
+
+*)
+
+(*Exp app 
+ input f:Exp(A,B) ->Exp(C,D), g:A->B
+ output C->D.*)
+
+val Exap_def = qdefine_fsym("Exap",[‘f:Exp(A,B) -> Exp(C,D)’,‘g:A->B’])
+‘Tp0(f o Tp1(g))’ |> gen_all
+
+(*shift1(x):Exp(N,X) ->Exp(N,X) *)
+val shift1_uex = prove_store("shift1_uex",
+e0
+(cheat)
+(form_goal “!x:1->X.?!f:Exp(N,X) ->Exp(N,X).
+ !g:N ->X. Exap(f,g) o O = x & !n:1->N.Exap(f,g) o Suc(n) = g o n”));
+
+val shift1_def = shift1_uex |> spec_all |> uex2ex_rule 
+                            |> qSKOLEM "shift1" [‘x’] 
+
+val llf_uex = prove_store("llf_uex",
+e0
+(cheat)
+(form_goal
+ “?!f: Exp(Exp(N,A+1),1+1) -> Exp(Exp(N,A+1),1+1).
+  !gs:1-> Exp(Exp(N,A+1),1+1) g.
+  IN(g,f o gs) <=>
+  g = Tp1(i2(A,1) o To1(N)) |
+  ?h t. g  = shift1(i1(A,1) o h) o t & IN(t,gs)”));
+
+val llf_def = llf_uex |> uex2ex_rule |> qSKOLEM "llf" [‘A’]
+                      |> gen_all
+
+val llf_monotone = prove_store("llf_monotone",
+e0
+cheat
+(form_goal “monotone(llf(A))”));
+
+val islls_def = qdefine_fsym("islls",[‘A’]) ‘gfp(llf(A))’
+
+val llist_def1 = Thm_2_4 |> qsspecl [‘Tp0(islls(X))’]
+                              |> qSKOLEM "llist" [‘X’] 
+                              |> qSKOLEM "repll" [‘X’]
+                              |> gen_all 
+
+val repll_Inj = llist_def1 |> spec_all 
+                          |> conjE1 |> gen_all
+                          |> store_as "repll_Inj"; 
+
+val ll_rules = rules0 |> gen_all |> qsspecl [‘llf(A)’] 
+                       |> C mp llf_monotone 
+                       |> rewr_rule[SS_def,llf_def] 
+                       |> mk_rules2 |> mk_rules3
+                       |> rewr_rule[GSYM islls_def]
+                       |> gen_all
+
+val ll_coind = coind0 |> gen_all |> qspecl [‘Exp(N,A + 1)’,‘llf(A)’]
+                      |> rewr_rule[SS_def,llf_def]
+                      |> rewr_rule[GSYM islls_def]
+                      |> gen_all
+
+val ll_cases = cases0 |> gen_all |> qsspecl [‘llf(A)’] 
+                      |> C mp llf_monotone
+                      |> rewr_rule[GSYM IN_EXT,llf_def]
+                      |> rewr_rule[GSYM islls_def]
+                      |> gen_all
+
+val isll_def = qdefine_psym("isll",[‘l:1->Exp(N,X + 1)’]) 
+                          ‘IN(l,islls(X))’
+                          |> gen_all |> store_as "isll_def"; 
+
+val isll_coinduct = ll_coind |> rewr_rule[IN_Tp0] 
+                             |> qsspecl [‘Tp1(P:Exp(N, X + 1)-> 2)’]
+                             |> rewr_rule[Tp0_Tp1_inv]
+                             |> rewr_rule[GSYM IN_Tp0,GSYM isll_def]
+                             |> gen_all
+
+val isll_lnil = prove_store("isll_lnil",
+e0
+(rw[isll_def,ll_rules])
+(form_goal
+ “!X. isll(Tp1(i2(X, 1) o To1(N)))”)); 
+
+
+val isll_shift = ll_rules |> spec_all |> conjE2 
+                        |> rewr_rule[GSYM isll_def]
+                        |> spec_all |> undisch 
+                        |> gen_all |> disch_all
+                        |> gen_all |> store_as "isll_shift";
+
+
+val Repll_def = qdefine_fsym ("Repll",[‘l:1-> llist(X)’])
+                            ‘repll(X) o l’
+                            |> gen_all |> store_as "Repll_def";
+ 
+val llist_def = llist_def1 |> rewr_rule[GSYM IN_Tp1,Tp1_Tp0_inv]
+                         |> gen_all
+                         |> store_as "llist_def";
+
+
+val LNil_def = proved_th $
+e0
+(strip_tac >> uex_tac >>
+ qspecl_then [‘X’] strip_assume_tac llist_def >>
+ first_assum (qspecl_then [‘Tp1(i2(X, 1) o To1(N))’] assume_tac) >>
+ fs[isll_lnil,GSYM isll_def] >>
+ qexists_tac ‘b’ >> arw[Repll_def] >>
+ fs[Inj_def])
+(form_goal “!X. ?!l.Repll(l) = Tp1(i2(X, 1) o To1(N))”)
+|> spec_all |> uex2ex_rule |> qSKOLEM "LNil" [‘X’] |> gen_all
+|> store_as "LNil_def";
+
+
+val lcons0_def = 
+    qdefine_fsym ("lcons0",[‘x:1->X’,‘l:1->Exp(N,X + 1)’])
+    ‘shift1((i1(X, 1) o x)) o l’ |> qgenl [‘X’,‘x’,‘l’]
+
+
+val lcons1_def = proved_th $
+e0
+cheat
+(form_goal “?!lcons1:X * Exp(N,X + 1) -> Exp(N,X+1).!x l.
+ lcons1 o Pa(x,l) = lcons0(x,l)”)
+|> uex2ex_rule |> qSKOLEM "lcons1" [‘X’] |> gen_all
+
+
+val repll_isll = prove_store("repll_isll",
+e0
+(rpt strip_tac >> 
+ rw[isll_def] >> 
+ qspecl_then [‘X’] assume_tac llist_def >>
+ fs[] >> qexists_tac ‘ll’ >> rw[])
+(form_goal “!X ll. isll(repll(X) o ll)”)); 
+
+
+val isll_Repll = llist_def |> spec_all |> conjE2
+                        |> rewr_rule[GSYM isll_def,
+                                     GSYM Repll_def] 
+                        |> gen_all 
+                        |> store_as "isll_Repll";
+
+
+val llift_cond2 = proved_th $
+e0
+(fconv_tac forall_cross_fconv >>
+ rw[Prla_def,Pa_distr,o_assoc,
+    p12_of_Pa,idL,lcons1_def] >>
+ rpt strip_tac >>
+ qsspecl_then [‘b’] assume_tac repll_isll >>
+ drule isll_shift >> rw[GSYM Repll_def,GSYM isll_Repll] >>
+ fs[Repll_def,lcons0_def])
+(form_goal
+ “!xl1:1-> X * llist(X).?l2.
+ (lcons1(X) o Prla(id(X),repll(X))) o xl1 = repll(X) o l2”)
+
+
+val llift_cond2' = proved_th $
+e0
+(assume_tac llift_cond2 >> strip_tac >> uex_tac >>
+ first_x_assum (qspecl_then [‘xl1’] strip_assume_tac) >>
+ qexists_tac ‘l2’ >> arw[] >> assume_tac repll_Inj >>
+ fs[Inj_def] >> rpt strip_tac >> first_x_assum irule >> arw[])
+(form_goal
+ “!xl1:1-> X * llist(X).?!l2.
+ (lcons1(X) o Prla(id(X),repll(X))) o xl1 = repll(X) o l2”)
+
+
+val LCONS_def = P2fun' |> qspecl [‘X * llist(X)’,‘llist(X)’]
+                     |> specl [qform2IL [‘xl1:1->X * llist(X)’,‘l2:1-> llist(X)’]
+ ‘(lcons1(X) o Prla(id(X),repll(X))) o xl1 = repll(X) o l2’]
+                     |> rewr_rule[Holds_def]
+                     |> rewr_rule[Eq_property_TRUE,o_assoc,
+                                 Pa_distr ,p12_of_Pa]
+                     |> C mp (llift_cond2' |> rewr_rule[o_assoc])
+                     |> uex2ex_rule
+                     |> qSKOLEM "LCONS" [‘X’]
+                     |> qspecl 
+                     [‘Pa(x:1->X,l:1-> llist(X))’]
+                     |> rewr_rule[Prla_def,
+                                  p12_of_Pa,idL,Pa_distr,
+                                  o_assoc,lcons1_def,lcons0_def,GSYM Repll_def]
+                     |> gen_all
+                     |> store_as "LCONS_def"; 
+
+val LCons_def = 
+    qdefine_fsym ("LCons",[‘x:1->X’,‘l:1->llist(X)’])
+    ‘LCONS(X) o Pa(x,l)’ 
+    |> gen_all |> store_as "LCons_def";
+
+val Repll_LCons = LCONS_def |> rewr_rule[GSYM LCons_def]
+                         |> GSYM
+                         |> store_as "Repll_LCons";
+
+
+
+val Repll_eq_eq = prove_store("Repll_eq_eq",
+e0
+(rpt strip_tac >> rw[Repll_def] >> irule Inj_eq_eq >>
+ rw[repll_Inj])
+(form_goal “!X l1:1->llist(X) l2.
+ Repll(l1) = Repll(l2) <=> l1 = l2”));
+
+val Ev_eq_eq' = prove_store("Ev_eq_eq'",
+e0
+(rpt strip_tac >> dimp_tac >> strip_tac >> arw[]>> 
+ drule Ev_eq_eq >> arw[])
+(form_goal “!A B X f:X->Exp(A,B) g. 
+ Ev(A,B) o Pa(p1(A,X),f o p2(A,X)) = 
+ Ev(A,B) o Pa(p1(A,X),g o p2(A,X)) <=> f = g”));
+
+
+val Ev_eq_eq' = prove_store("Ev_eq_eq'",
+e0
+(rpt strip_tac >> dimp_tac >> strip_tac >> arw[]>> 
+ drule Ev_eq_eq >> arw[])
+(form_goal “!A B X f:X->Exp(A,B) g. 
+ Ev(A,B) o Pa(p1(A,X),f o p2(A,X)) = 
+ Ev(A,B) o Pa(p1(A,X),g o p2(A,X)) <=> f = g”));
+
+val Tp0_eq_eq = prove_store("Tp0_eq_eq",
+e0
+(cheat)
+(form_goal “!A B f:1->Exp(A,B) g. Tp0(f) = Tp0(g) <=> f = g”));
+
+
+val Tp1_eq_eq = prove_store("Tp1_eq_eq",
+e0
+(cheat)
+(form_goal “!A B f:A->B g. Tp1(f) = Tp1(g) <=> f = g”));
+
+val i12_disjoint = prove_store("i12_disjoint",
+e0
+cheat
+(form_goal “!A B a:1->A b:1->B. ~(i1(A,B) o a = i2(A,B) o b)”));
+
+val LCons_NONLNIL = prove_store("LCons_NONLNIL",
+e0
+(rw[GSYM Repll_eq_eq,LNil_def,Repll_LCons] >>
+ rpt strip_tac >> rw[GSYM Tp0_eq_eq] >>
+ rw[Tp0_Tp1_inv] >> once_rw[GSYM FUN_EXT_iff] >>
+ ccontra_tac >>
+ first_x_assum (qspecl_then [‘O’] assume_tac) >>
+ fs[o_assoc,one_to_one_id,idR] >>
+ qby_tac ‘Tp0((shift1((i1(X, 1) o x)) o Repll(l))) o O = 
+  Exap(shift1(i1(X, 1) o x),Tp0(Repll(l))) o O’
+ >-- rw[Exap_def,Tp1_Tp0_inv] >>
+ fs[shift1_def] >>
+ qsspecl_then [‘x’,‘id(1)’] assume_tac i12_disjoint >>
+ fs[idR])
+(form_goal
+ “!X x l. ~(LCons(x,l) = LNil(X))”));
+
+
+
+val Repll_lnil_uex = prove_store("Repl_lnil_uex",
+e0
+(rpt strip_tac >> dimp_tac >> strip_tac >> arw[LNil_def] >>
+ rw[GSYM Repll_eq_eq] >> arw[LNil_def])
+(form_goal
+ “!X l. Repll(l) = Tp1(i2(X, 1) o To1(N)) <=> l = LNil(X)”));
+
+
+
+val _ = new_psym2IL("isll",(rastt "Tp0(islls(X))",List.map (dest_var o rastt) ["nxs:A->Exp(N,X+1)"]))
+
+val _ = new_fsym2IL("Repll",(rastt "repll(X)",List.map (dest_var o rastt) ["l:A-> llist(X)"]))
+
+val lnil_def = qdefine_fsym("lnil",[‘X’]) ‘Tp1(i2(X, 1) o To1(N))’
+
+(*\cal B*)
+val CB_def = proved_th $
+e0
+cheat
+(form_goal “!X. ?!f:Exp(Exp(N,X+1) * Exp(N,X+1) ,1+1) ->
+                    Exp(Exp(N,X+1) * Exp(N,X+1),1+1).
+ !g1 g2 R. IN(Pa(g1,g2),f o R) <=>
+ (g1 = lnil(X) & g2 = lnil(X)) | 
+ ?f1 f2 x. IN(Pa(f1,f2),R) & g1 = lcons0(x,f1) & g2 = lcons0(x,f2) & 
+ isll(f1) & isll(f2)”)
+|> spec_all |> uex2ex_rule |> qSKOLEM "CB" [‘X’]
+
+
+(*
+> > > > > # 1 subgoal:
+val it =
+   X(g2 : ar(1, Exp(N, X + 1)))(g1 : ar(1, Exp(N, X + 1)))(X' :
+      ar(1, Exp(Exp(N, (X + 1)) * Exp(N, (X + 1)), 2)))
+   1.!(a' : ar(1, Exp(N, X + 1)))  (b : ar(1, Exp(N, X + 1))).
+               IN(Pa(a'#, b#), X') ==>
+               a'# = lnil(X) & b# = lnil(X) |
+               ?(f1 : ar(1, Exp(N, X + 1)))  (f2 : ar(1, Exp(N, X + 1)))
+               (x1 : ar(1, X))  (x2 : ar(1, X)).
+                 IN(Pa(f1#, f2#), X') &
+                 a'# = lcons0(x1#, f1#) &
+                 b# = lcons0(x2#, f2#) & isll(f1#) & isll(f2#)
+   2.IN(Pa(g1, g2), X')
+   3.isll(g1) & isll(g2)
+   4.~g1 = g2
+   ----------------------------------------------------------------------
+   F
+
+*)
+
+val NTC0_def = proved_th $
+e0
+cheat
+(form_goal “?NTC:N * Exp(N,X+1) -> Exp(N,X+1).!n0 g0.
+  (!n. Le(n,n0) ==> Tp0(NTC o Pa(n0,g0)) o n = Tp0(g0) o n) & 
+  (!n. ~(Le(n,n0)) ==> Tp0(NTC o Pa(n0,g0)) o n = i2(X,1))”)
+|> qSKOLEM "NTC0" [‘X’]
+
+val ntc0_def = qdefine_fsym("ntc0",[‘n:1->N’,‘g:1->Exp(N,X+1)’])
+‘NTC0(X) o Pa(n,g)’
+
+val ntc0_eq_eq = prove_store("ntc_eq_eq",
+e0
+cheat
+(form_goal “!g1 g2:1->Exp(N,X+1). isll(g1) & isll(g2) & 
+ (!n. ntc0(n,g1) = ntc0(n,g2)) ==> g1 = g2”));
+
+val ntc0_lcons0 = prove_store("ntc0_lcons0",
+e0
+(cheat)
+(form_goal “!n x f. ntc0(Suc(n), lcons0(x, f)) = 
+shift1(i1(X,1) o x) o ntc0(n,f)”));
+
+(*proved_th $
+e0
+cheat
+(form_goal
+ “!n0:1->N g0:1->Exp(N,X+1).?!g:1->Exp(N,X + 1).
+  (!n. Le(n,n0) ==> Tp0(g) o n = Tp0(g0) o n) & 
+  (!n. ~(Le(n,n0)) ==> Tp0(g) o n = i2(X,1))”)*)
+
+
+
+
+val CB_monotone = prove_store("CB_monotone",
+e0
+cheat
+(form_goal “monotone(CB(X))”));
+
+
+
+(*P ⊆ A, ϕ: A -> X * A g: A -> LL(X)*)
+
+val llindf_def = proved_th $
+e0
+cheat
+(form_goal “!A P:1->Exp(A,1+1) phi:A -> X * A.
+ ?!f:Exp(A * llist(X),1+1) -> Exp(A * llist(X),1+1).
+ !s:1-> Exp(A * llist(X),1+1).
+  !p:1->A * llist(X). 
+  IN(p, f o s) <=>
+  (IN(Fst(p),P) & Snd(p)= LNil(X)) |
+  (?p0:1->A * llist(X). IN(p0,s) &
+   ~IN(Fst(p),P) & Snd(phi o Fst(p)) = Fst(p0) &
+   Snd(p) = LCons(Fst(phi o Fst(p)), Snd(p0)))”)
+ |> spec_all |> uex2ex_rule |> qSKOLEM "llindf"[‘P’,‘phi’]
+
+
+val llindf_monotone = prove_store("llindf_monotone",
+e0
+cheat
+(form_goal “monotone(llindf(P:1->Exp(A,1+1),phi:A->X * A))”));
+
+
+val llinds_def = qdefine_fsym("llinds",[‘P:1->Exp(A,1+1)’,‘phi:A->X * A’])
+‘gfp(llindf(P, phi))’
+
+
+val llind_rules  = rules0 |> gen_all |> qsspecl [‘llindf(P:1->Exp(A,1+1),phi:A->X * A)’] 
+                       |> C mp llindf_monotone 
+                       |> rewr_rule[SS_def,llindf_def] 
+                       |> rewr_rule[GSYM llinds_def]
+                       |> mk_rules2 |> mk_rules3
+                       |> gen_all
+
+val llind_coind = coind0 |> gen_all |> qspecl [‘A * llist(X)’,‘llindf(P:1->Exp(A,1+1),phi:A->X * A)’]
+                      |> rewr_rule[SS_def,llindf_def]
+                      |> rewr_rule[GSYM llinds_def]
+                      |> gen_all
+
+
+val CB_cases = cases0 |> gen_all |> qsspecl [‘CB(X)’] 
+                      |> C mp CB_monotone
+                      |> rewr_rule[GSYM IN_EXT]
+                      |> conv_rule (depth_fconv no_conv forall_cross_fconv)
+                      |> rewr_rule[CB_def]
+                      |> gen_all
+
+
+val CB_rules  = rules0 |> gen_all |> qsspecl [‘CB(X)’] 
+                       |> C mp CB_monotone 
+                       |> rewr_rule[SS_def] 
+                       |> conv_rule (depth_fconv no_conv forall_cross_fconv)
+                       |> rewr_rule[CB_def]
+                       |> mk_rules2 |> mk_rules3
+                       |> gen_all
+
+val CB_coind = coind0 |> gen_all |> qspecl [‘Exp(N,X+1) * Exp(N,X+1)’,‘CB(X)’]
+                      |> rewr_rule[SS_def]
+                      |> conv_rule (depth_fconv no_conv forall_cross_fconv)
+                      |> rewr_rule[CB_def]
+                      |> gen_all
+
+
+val llind_cases = cases0 |> gen_all |> qsspecl [‘llindf(P:1->Exp(A,1+1),phi:A->X * A)’] 
+                      |> C mp llindf_monotone
+                      |> rewr_rule[GSYM IN_EXT,llindf_def]
+                      |> rewr_rule[GSYM llinds_def]
+                      |> gen_all
+
+val gfp_CB = prove_store("gfp_CB",
+e0
+cheat
+(form_goal
+“!X g1 g2. IN(Pa(g1,g2),gfp(CB(X))) <=> (g1 = g2 &  isll(g1) & isll(g2))”));
+
+val CB_coind1 = CB_coind |> rewr_rule[gfp_CB]
+
+“?f:Exp(A,1+1) * Exp(B,1+1) -> !sa:1->Exp(A,1+1) sb:1->Exp(B,1+1).
+ ”
+
+rpt strip_tac >>
+irule $ iffLR Repll_eq_eq >>
+qsuff_tac ‘Repll(ll1) = Repll(ll2) & isll(Repll(ll1)) & isll(Repll(ll2))’
+>-- (strip_tac >> arw[]) >>
+irule CB_coind1 >>
+qby_tac
+‘?s:1->Exp(Exp(N, (X + 1)) * Exp(N, (X + 1)), 1+1). 
+ ’
+
+
+qexists_tac ‘Pa(llinds(P, phi),llinds(P, phi))’
+llind_cases 
+“!a:1->A.!ll1:1->llist(X) ll2.IN(Pa(a,ll1),llinds(P,phi)) &
+ IN(Pa(a,ll2),llinds(P,phi)) ==> ll1 = ll2”
+
+
+(*if a in P then the unique ll is [], 
+ else a is hit by some snd of phi:A->X * A.
+
+
+
+If P ⊆ X and ϕ : X → N × X, then g : X → L *)
+
+
+
+“!a:1->A.?!ll:1->llist(X).IN(Pa(a,ll),llinds(P,phi)) ”
+
+
+
+(*
+
+⊢ ∀f z.
+       LUNFOLD f z =
+       llist_abs
+         (λn.
+              OPTION_MAP SND
+                (FUNPOW (λm:(β#α)opt. OPTION_BIND m (UNCURRY (K ∘ f))) n (f z))):
+
+
+ "LUNFOLD",
+  `!f x.
+     LUNFOLD f:β->(β #a) opt x:β =
+       case f x of NONE => [||] | SOME (v1,v2) => v2 ::: LUNFOLD f v1`
+
+val it =
+   ⊢ (∀f x. OPTION_MAP f:α->β (SOME x) = SOME (f x)) ∧
+     ∀f. OPTION_MAP f NONE = NONE
+
+
+(∀f. OPTION_BIND NONE f:β->α opt = NONE) ∧ ∀x f. OPTION_BIND (SOME x) f = f x
+
+
+("arithmetic", "FUNPOW"),
+     (⊢ (∀f x. FUNPOW f 0 x = x) ∧
+        ∀f n x. FUNPOW f (SUC n) x = FUNPOW f n (f x), Def))
+
+“!g1 g2 n. IN(Pa(g1,g2),gfp(CB(X))) ==> ntc0(n,g1) =  ntc0(n,g2)”
+rw[IN_gfp] >> rpt strip_tac >> rw[SS_def] >>
+fconv_tac (depth_fconv no_conv forall_cross_fconv) >>
+rw[CB_def] >> dimp_tac >> strip_tac (* 2 *) >-- 
+qby_tac ‘!n f1 f2.IN(Pa(f1,f2),X') ==> ntc0(n,f1) = ntc0(n,f2)’
+>-- qsuff_tac ‘!n. (!n0. Lt(n0,n) ==> !f1 f2.IN(Pa(f1,f2),X') ==> ntc0(n0,f1) = ntc0(n0,f2)) ==> !f1 f2.IN(Pa(f1,f2),X') ==> ntc0(n,f1) = ntc0(n,f2)’
+    >-- cheat >> 
+rpt strip_tac >>
+first_assum drule >> pop_assum strip_assume_tac >-- cheat >>
+arw[] >> 
+cheat
+
+
+rpt strip_tac >> dimp_tac >-- cheat >>
+rpt strip_tac >> arw[] >> rw[IN_gfp] >> 
+
+qsuff_tac ‘!n0. Le(n0,n) ==>  ntc0(n0, f1) = ntc0(n0, f2)’
+>-- cheat >>
+
+qsuff_tac ‘!n0. Le(n0,n) ==> Tp0(f1) o n0 = Tp0(f2) o n0’     
+>-- cheat >>
+rpt strip_tac >>
+qcases ‘n0 = n’ >> arw[] >>
+first_assum drule >> pop_assum strip_assume_tac >-- cheat (*Nil trivial*) >>
+
+
+
+
+>-- rpt strip_tac >>
+    qsuff_tac ‘!n.(!n0.Lt(n0,n) ==> ntc0(n0, f1) = ntc0(n0, f2)) ==>
+                ntc0(n, f1) = ntc0(n, f2)’
+    >-- cheat >>
+    rpt strip_tac >> first_assum drule >>
+    pop_assum strip_assume_tac >-- cheat >>
+    
+
+
+qsuff_tac ‘isll(g1) & isll(g2)’ >-- 
+strip_tac >> arw[] >> irule ntc0_eq_eq >> arw[] >>
+qsuff_tac ‘ntc0(O,g1) = ntc0(O,g2) & IN(Pa(ntc0(O,g1),ntc0(O,g2)),X') &
+ (!n0. ntc0(n0,g1) = ntc0(n0,g2) & IN(Pa(ntc0(n0,g1),ntc0(n0,g2)),X') ==>
+ ntc0(Suc(n0),g1) = ntc0(Suc(n0),g2) &
+  IN(Pa(ntc0(Suc(n0),g1),ntc0(Suc(n0),g2)),X'))’
+>-- cheat >>
+strip_tac >-- cheat >> strip_tac >-- cheat >>
+strip_tac >> disch_tac >>
+
+
+
+
+cheat  >>
+strip_tac >> irule ll_coind >> cheat
+
+
+
+>-- disch_tac >> arw[] >> 
+    qsuff_tac ‘!n. ntrunc g1 = ntrunc g2 & isll(ntrunc g1) & isll(ntrunc g2)’
+    induct on n
+   Nil = Nil
+   assume ntrunc n g1 = ntrunc n g2 & isll(ntrunc n g1) & isll(ntrunc n g2)
+want 
+
+“!g1 g2. IN(Pa(g1,g2),gfp(CB(X))) <=> (g1 = g2 &  isll(g1) & isll(g2))”
+
+coind0 |> gen_all |> qspecl [‘Exp(N,X + 1) * Exp(N,X + 1)’,‘CB(X)’]
+|> rewr_rule[SS_def]
+|> conv_rule  (depth_fconv no_conv forall_cross_fconv) 
+|> rewr_rule[CB_def]
+
+cases0 |> gen_all |> qsspecl [‘CB(X)’] 
+|> C mp CB_monotone
+|> rewr_rule[GSYM IN_EXT,CB_def]
+|> conv_rule (depth_fconv no_conv forall_cross_fconv) 
+|> rewr_rule[CB_def]
+
+(*
+(form_goal “!X. ?!f:Pow(llist(X) * llist(X)) -> Pow(llist(X) * llist(X)).
+ !a1 a2 a3 a4. IN(Pa(a3,a4),f o Pa(a1,a2)) <=> 
+ a3 = LNil(X) & a4 = LNil(X) & ...
+ ”) cannot define like this since must be Exp 
+*)
+
+
+
+
+“?form conj: form * form -> form disj:form -> form > form neg:form ->form
+ imp:form * form ->form diam:form -> form.
+ 
+”
+prove_store("isL_coinduct",
+e0
+(rw[isll_def] >> strip_tac >> strip_tac >>
+ qsspecl_then [‘Tp1(P)’] assume_tac ll_coind >>
+ fs[IN_Tp1])
+(form_goal 
+ “!X P.P o Tp1(i2(X, 1) o To1(N))  = TRUE & 
+  (!lls0 x. P o lls0 = TRUE ==>
+    P o Ins(Pa(Card(ls0),x),ls0) = TRUE) ==> 
+  !l:1-> Exp(N * X,1+1). isL(l) ==> P o l = TRUE”));
+
+
+
+ "LTAKE_SNOC_LNTH",
+  ``!n ll. LTAKE (SUC n) ll =
+             case LTAKE n ll of
+               NONE => NONE
+             | SOME l => (case LNTH n ll of
+                             NONE => NONE
+                           | SOME e => SOME (l ++ [e]))``
+
+ "LTAKE_EQ_NONE_LNTH",
+  ``!n ll. (LTAKE n ll = NONE) ==> (LNTH n ll = NONE)``
+
+  "LNTH_EQ",
+  ``!ll1 ll2. (ll1 = ll2) = (!n. LNTH n ll1 = LNTH n ll2)``
+
+ "LTAKE_EQ",
+  ``!ll1 ll2. (ll1 = ll2) = (!n. LTAKE n ll1 = LTAKE n ll2)``
+
+
+*)
