SEARrecty.sml
@@ -1,0 +1,126 @@
+(*Udef can only be abbrev since no set equality*)
+
+val InjN_def = proved_th $
+e0
+(cheat)
+(form_goal “!A. ?!injN:N -> Pow(N * A).
+ !n0. (!n a.IN(Pair(n,a),App(injN,n0)) <=> n = n0)”)
+|> spec_all |> uex2ex_rule |> qSKOLEM "InjN" [‘A’] |> gen_all 
+
+
+val InjA_def = proved_th $
+e0
+(cheat)
+(form_goal “!A. ?!injA:A -> Pow(N * A).
+ !a0. (!n a.IN(Pair(n,a),App(injA,a0)) <=> a = a0)”)
+|> spec_all |> uex2ex_rule |> qSKOLEM "InjA" [‘A’] |> gen_all 
+
+val Even_def = qdefine_psym("Even",[‘n:mem(N)’]) ‘∃n0. n = Mul(Suc(Suc(O)),n0)’
+val Odd_def = qdefine_psym("Odd",[‘n:mem(N)’]) ‘~Even(n)’
+
+(*pretend we have div*)
+val DIV2_def = proved_th $
+e0
+cheat
+(form_goal “∃!f:N ->N. (∀n.Even(n) ⇔ App(f,n) = O) &
+ (∀n. Odd(n) ⇔ App(f,n) = Suc(O)) ”)
+|> uex2ex_rule |> qSKOLEM "DIV2" []
+
+val Div_def = qdefine_fsym("Div2",[‘n:mem(N)’]) ‘App(DIV2,n)’
+
+                          
+val InjUU_def = proved_th $
+e0
+cheat
+(form_goal “∀A.∃!f:Pow(N * A) * Pow(N * A) -> Pow(N * A).
+ ∀u1 u2. ∀n a. IN(Pair(n,a),App(f,Pair(u1,u2))) ⇔ 
+  ((Even(n) & IN(Pair(Div2(n),a),u1)) | 
+   (Odd(n) & IN(Pair(Div2(n),a),u2)))”)
+|> spec_all |> uex2ex_rule |> qSKOLEM "InjUU" [‘A’]
+
+val injN_def = qdefine_fsym("injN",[‘A’,‘n:mem(N)’]) ‘App(InjN(A),n)’
+val injA_def = qdefine_fsym("injA",[‘a:mem(A)’]) ‘App(InjA(A),a)’ 
+val injUU_def = 
+    qdefine_fsym("injUU",[‘u1:mem(Pow(N * A))’,‘u2:mem(Pow(N * A))’]) 
+                ‘App(InjUU(A),Pair(u1,u2))’ 
+
+
+
+val num1_def = qdefine_fsym("num1",[]) ‘Suc(O)’
+val num2_def = qdefine_fsym("num2",[]) ‘Suc(num1)’
+val num3_def = qdefine_fsym("num3",[]) ‘Suc(num2)’
+val num4_def = qdefine_fsym("num4",[]) ‘Suc(num3)’
+
+(*FALSE *)
+val F0_def = qdefine_fsym("F0",[‘A’]) ‘injN(A,O)’
+
+val VAR0_def = qdefine_fsym("VAR0",[‘A’]) ‘InjUU(A) o Pa(El(injN(A,num1)) o To1(A),InjA(A))’
+
+val Var0_def = qdefine_fsym("Var0",[‘a:mem(A)’]) ‘App(VAR0(A),a)’
+
+val NEG0_def = qdefine_fsym("NEG0",[‘A’]) ‘InjUU(A) o 
+Pa(El(injN(A,num2)) o To1(Pow(N * A)),Id(Pow(N * A)))’
+
+
+val Neg0_def = qdefine_fsym("Neg0",[‘f0:mem(Pow(N * A))’]) ‘App(NEG0(A),f0)’
+
+ 
+val DISJ0_def = qdefine_fsym("DISJ0",[‘A’]) ‘InjUU(A) o 
+Pa(El(injN(A,num3)) o To1(Pow(N * A) * Pow(N * A)),InjUU(A))’
+
+val Disj0_def = qdefine_fsym("Disj0",[‘f1:mem(Pow(N * A))’,‘f2:mem(Pow(N * A))’]) ‘App(DISJ0(A),Pair(f1,f2))’
+
+val DIAM0_def = qdefine_fsym("DIAM0",[‘A’])
+‘InjUU(A) o 
+Pa(El(injN(A,num4)) o To1(Pow(N * A)),Id(Pow(N * A)))’
+
+val Diam0_def = qdefine_fsym("Diam0",[‘f0:mem(Pow(N * A))’]) ‘App(DIAM0(A),f0)’
+
+
+
+val f = 
+ “(nas = F0 ==> IN(nas,isfms)) &
+  (!p:mem(A). nas = Var0(p) ⇒ IN(nas,isfms)) &
+  (∀f0.IN(f0,isfms) & nas = Neg0(f0) ⇒ IN(nas,isfms)) & 
+  (∀f1 f2.IN(f1,isfms) & IN(f2,isfms) & nas = Disj0(f1,f2) ⇒ IN(nas,isfms)) &
+  (∀f0.IN(f0,isfms) & nas = Diam0(f0) ⇒ IN(nas,isfms))”
+
+
+val isfm_cl = 
+  “(nas = F0(A) ==> IN(nas,isfms)) &
+  (!p:mem(A). nas = Var0(p) ⇒ IN(nas,isfms)) &
+  (∀f0.IN(f0,isfms) & nas = Neg0(f0) ⇒ IN(nas,isfms)) & 
+  (∀f1 f2.IN(f1,isfms) & IN(f2,isfms) & nas = Disj0(f1,f2) ⇒ IN(nas,isfms)) &
+  (∀f0.IN(f0,isfms) & nas = Diam0(f0) ⇒ IN(nas,isfms))”
+
+val (isfm_incond,x1) = mk_incond isfm_cl;
+val isfmf_ex = mk_fex isfm_incond x1;
+val isfmf_def = mk_fdef "isfmf" isfmf_ex;
+val isfmf_monotone = mk_monotone isfmf_def;
+val isfm's_def = mk_prim isfmf_def;
+val isfms_def = mk_LFP (rastt "isfm's(A)");
+val isfms_cond = mk_cond isfms_def isfm's_def;
+val isfms_SS = mk_SS isfms_def isfm's_def;
+val isfm_rules0 = mk_rules isfmf_monotone isfms_SS isfms_cond;
+val isfm_cases0 = mk_cases isfmf_monotone isfm_rules0 isfms_cond;
+val isfm_ind0 = mk_ind isfms_cond;
+val isfm_ind1 = mk_ind1 isfmf_def isfm_ind0;
+val isfm_ind2 = mk_ind2 isfm_ind1;
+val isfm_cases1 = mk_case1 isfmf_def isfm_cases0;
+val isfm_rules1 = mk_rules1 isfmf_def isfm_rules0;
+val isfm_rules2 = mk_rules2 isfm_rules1;
+val isfm_rules3 = mk_rules3 isfm_rules2;
+
+
+
+
+val isfm_ind = isfm_ind2 |> store_as "isfm_ind";
+val isfm_cases = isfm_cases1 |> store_as "isfm_cases";
+val isfm_rules = isfm_rules3 |> store_as "isfm_rules";
+
+
+(*model is a R:A~>A with a member of Pow(A * N)
+
+type of model: Pow(A * A) * Pow(A * N)
+ *)
+
